src/tls/Format.fst
@@ -1,0 +1,259 @@
+module Format
+
+open FStar.All
+
+open FStar.Seq
+open Platform.Bytes
+open Platform.Error
+open TLSError
+
+module HH = FStar.HyperHeap
+module HS = FStar.HyperStack
+
+// TLS memory---an attempt at splitting TLSConstants
+
+(** Regions and colors for objects in memory *)
+let tls_color = -1
+let epoch_color = 1
+let hs_color = 2
+
+let is_tls_rgn r   = HH.color r = tls_color
+let is_epoch_rgn r = HH.color r = epoch_color
+let is_hs_rgn r    = HH.color r = hs_color
+
+(*
+ * AR: Adding the eternal region predicate.
+ * Strengthening the predicate because at some places, the code uses HH.parent.
+ *)
+let rgn       = r:HH.rid{r<>HH.root
+                         /\ (forall (s:HH.rid).{:pattern HS.is_eternal_region s} HS.is_above s r ==> HS.is_eternal_region s)}
+let tls_rgn   = r:rgn{is_tls_rgn r}
+let epoch_rgn = r:rgn{is_epoch_rgn r}
+let hs_rgn    = r:rgn{is_hs_rgn r}
+
+let tls_region : tls_rgn = new_colored_region HH.root tls_color
+
+let tls_tables_region : (r:tls_rgn{HH.parent r = tls_region}) =
+    new_region tls_region
+
+
+
+// basic parsing and formatting---an attempt at splitting TLSConstant.
+
+type pinverse_t (#a:Type) (#b:Type) ($f:(a -> Tot b)) = b -> Tot (result a)
+
+unfold type lemma_inverse_g_f (#a:Type) (#b:Type) ($f:a -> Tot b) ($g:b -> Tot (result a)) (x:a) =
+  g (f x) == Correct x
+
+unfold type lemma_pinverse_f_g (#a:Type) (#b:Type) (r:b -> b -> Type) ($f:a -> Tot b) ($g:b -> Tot (result a)) (y:b) =
+  Correct? (g y) ==> r (f (Correct?._0 (g y))) y
+
+
+(** Transforms a sequence of natural numbers into bytes *)
+val bytes_of_seq: n:nat{ repr_bytes n <= 8 } -> Tot (b:bytes{length b <= 8})
+let bytes_of_seq sn = bytes_of_int 8 sn
+
+(** Transforms bytes into a sequence of natural numbers *)
+val seq_of_bytes: b:bytes{ length b <= 8 } -> Tot nat
+let seq_of_bytes b = int_of_bytes b
+
+(** Transform and concatenate a natural number to bytes *)
+val vlbytes: lSize:nat -> b:bytes{repr_bytes (length b) <= lSize} -> Tot (r:bytes{length r = lSize + length b})
+let vlbytes lSize b = bytes_of_int lSize (length b) @| b
+
+(** Lemmas associated to bytes manipulations *)
+val lemma_vlbytes_len : i:nat -> b:bytes{repr_bytes (length b) <= i}
+  -> Lemma (ensures (length (vlbytes i b) = i + length b))
+let lemma_vlbytes_len i b = ()
+
+val lemma_vlbytes_inj : i:nat
+  -> b:bytes{repr_bytes (length b) <= i}
+  -> b':bytes{repr_bytes (length b') <= i}
+  -> Lemma (requires (Seq.equal (vlbytes i b) (vlbytes i b')))
+          (ensures (b == b'))
+let lemma_vlbytes_inj i b b' =
+  let l = bytes_of_int i (length b) in
+  Seq.lemma_append_inj l b l b'
+
+val vlbytes_length_lemma: n:nat -> a:bytes{repr_bytes (length a) <= n} -> b:bytes{repr_bytes (length b) <= n} ->
+  Lemma (requires (Seq.equal (Seq.slice (vlbytes n a) 0 n) (Seq.slice (vlbytes n b) 0 n)))
+        (ensures (length a = length b))
+let vlbytes_length_lemma n a b =
+  let lena = Seq.slice (vlbytes n a) 0 n in
+  let lenb = Seq.slice (vlbytes n b) 0 n in
+  assert(Seq.equal lena (bytes_of_int n (length a)));
+  assert(Seq.equal lenb (bytes_of_int n (length b)));
+  int_of_bytes_of_int n (length a); int_of_bytes_of_int n (length b)
+
+
+#set-options "--max_ifuel 1 --initial_ifuel 1 --max_fuel 0 --initial_fuel 0"   //need to reason about length
+
+
+val vlsplit: lSize:nat{lSize <= 4}
+  -> vlb:bytes{lSize <= length vlb}
+  -> Tot (result (b:(bytes * bytes){
+                    repr_bytes (length (fst b)) <= lSize
+                  /\ Seq.equal vlb (vlbytes lSize (fst b) @| (snd b))}))
+let vlsplit lSize vlb =
+  let (vl,b) = Platform.Bytes.split vlb lSize in
+  let l = int_of_bytes vl in
+  if l <= length b
+  then Correct(Platform.Bytes.split b l)
+  else Error(AD_decode_error, perror __SOURCE_FILE__ __LINE__ "")
+
+
+val vlparse: lSize:nat{lSize <= 4} -> vlb:bytes{lSize <= length vlb}
+  -> Tot (result (b:bytes{repr_bytes (length b) <= lSize /\ Seq.equal vlb (vlbytes lSize b)}))
+let vlparse lSize vlb =
+  let vl,b = split vlb lSize in
+  if int_of_bytes vl = length b
+  then Correct b
+  else Error(AD_decode_error, perror __SOURCE_FILE__ __LINE__ "")
+
+
+val vlparse_vlbytes: lSize:nat{lSize <= 4} -> vlb:bytes{repr_bytes (length vlb) <= lSize} -> Lemma
+  (requires (True))
+  (ensures (vlparse lSize (vlbytes lSize vlb) == Correct vlb))
+  [SMTPat (vlparse lSize (vlbytes lSize vlb))]
+let vlparse_vlbytes lSize vlb =
+  let vl,b = split (vlbytes lSize vlb) lSize in
+  assert (Seq.equal vl (bytes_of_int lSize (length vlb)));
+  int_of_bytes_of_int lSize (length vlb);
+  match vlparse lSize (vlbytes lSize vlb) with
+  | Error z   -> ()
+  | Correct b -> lemma_vlbytes_inj lSize vlb b
+
+
+// floating crypto definitions
+
+(** Finite Field Diffie-Hellman group definitions *)
+type ffdhe =
+  | FFDHE2048
+  | FFDHE3072
+  | FFDHE4096
+  | FFDHE6144
+  | FFDHE8192
+
+// BB.TODO: Document this !
+let _FFz = 0xFFz // Workaround for #514
+
+(** TLS 1.3 named groups for (EC)DHE key exchanges *)
+type namedGroup =
+  | SEC of CoreCrypto.ec_curve
+  | EC_UNSUPPORTED of (b:byte{b <> 0x17z /\ b <> 0x18z /\ b <> 0x19z})
+  | FFDHE of ffdhe
+  | FFDHE_PRIVATE_USE of (b:byte{b = 0xFCz \/ b = 0xFDz \/ b = 0xFEz \/ b = _FFz})
+  | ECDHE_PRIVATE_USE of byte
+
+(*
+ * We only seem to be using these two named groups
+ * irrespective of whether it's TLS 12 or 13
+ *)
+type valid_namedGroup = x:namedGroup{SEC? x \/ FFDHE? x}
+
+(** Serializing function for (EC)DHE named groups *)
+val namedGroupBytes: namedGroup -> Tot (lbytes 2)
+let namedGroupBytes ng =
+  let open CoreCrypto in 
+  match ng with
+  | SEC ec ->
+    begin
+    match ec with
+    | ECC_P256		-> abyte2 (0x00z, 0x17z)
+    | ECC_P384		-> abyte2 (0x00z, 0x18z)
+    | ECC_P521		-> abyte2 (0x00z, 0x19z)
+    end
+  | EC_UNSUPPORTED b	-> abyte2 (0x00z, b)
+  | FFDHE dhe ->
+    begin
+    match dhe with
+    | FFDHE2048		-> abyte2 (0x01z, 0x00z)
+    | FFDHE3072		-> abyte2 (0x01z, 0x01z)
+    | FFDHE4096		-> abyte2 (0x01z, 0x02z)
+    | FFDHE6144		-> abyte2 (0x01z, 0x03z)
+    | FFDHE8192		-> abyte2 (0x01z, 0x04z)
+    end
+  | FFDHE_PRIVATE_USE b -> abyte2 (0x01z, b)
+  | ECDHE_PRIVATE_USE b -> abyte2 (0xFEz, b)
+
+(** Parsing function for (EC)DHE named groups *)
+val parseNamedGroup: pinverse_t namedGroupBytes
+let parseNamedGroup b =
+  let open CoreCrypto in 
+  match cbyte2 b with
+  | (0x00z, 0x17z) -> Correct (SEC ECC_P256)
+  | (0x00z, 0x18z) -> Correct (SEC ECC_P384)
+  | (0x00z, 0x19z) -> Correct (SEC ECC_P521)
+  | (0x00z, b)     -> Correct (EC_UNSUPPORTED b) // REMARK: only values 0x01z-0x16z and 0x1Az-0x1Ez are assigned
+  | (0x01z, 0x00z) -> Correct (FFDHE FFDHE2048)
+  | (0x01z, 0x01z) -> Correct (FFDHE FFDHE3072)
+  | (0x01z, 0x02z) -> Correct (FFDHE FFDHE4096)
+  | (0x01z, 0x03z) -> Correct (FFDHE FFDHE6144)
+  | (0x01z, 0x04z) -> Correct (FFDHE FFDHE8192)
+  | (0x01z, b)     ->
+    if b = 0xFCz || b = 0xFDz || b = 0xFEz || b = 0xFFz
+    then Correct (FFDHE_PRIVATE_USE b)
+    else Error (AD_decode_error, perror __SOURCE_FILE__ __LINE__ "Wrong ffdhe private use group")
+  | (0xFEz, b)     -> Correct (ECDHE_PRIVATE_USE b)
+  | _ -> Error (AD_decode_error, perror __SOURCE_FILE__ __LINE__ "Wrong named group")
+
+(** Lemmas for named groups parsing/serializing inversions *)
+val inverse_namedGroup: x:_ -> Lemma
+  (requires (True))
+  (ensures lemma_inverse_g_f namedGroupBytes parseNamedGroup x)
+  [SMTPat (parseNamedGroup (namedGroupBytes x))]
+let inverse_namedGroup x = ()
+
+val pinverse_namedGroup: x:_ -> Lemma
+  (requires (True))
+  (ensures (lemma_pinverse_f_g Seq.equal namedGroupBytes parseNamedGroup x))
+  [SMTPat (namedGroupBytes (Correct?._0 (parseNamedGroup x)))]
+let pinverse_namedGroup x = ()
+
+
+private val namedGroupsBytes0: groups:list namedGroup
+  -> Tot (b:bytes { length b = op_Multiply 2 (List.Tot.length groups)})
+let rec namedGroupsBytes0 groups =
+  match groups with
+  | [] -> empty_bytes
+  | g::gs -> namedGroupBytes g @| namedGroupsBytes0 gs
+
+(** Serialization function for a list of named groups *)
+val namedGroupsBytes: groups:list namedGroup{List.Tot.length groups < 65536/2}
+  -> Tot (b:bytes { length b = 2 + op_Multiply 2 (List.Tot.length groups)})
+let namedGroupsBytes groups =
+  let gs = namedGroupsBytes0 groups in
+  lemma_repr_bytes_values (length gs);
+  vlbytes 2 gs
+
+private val parseNamedGroups0: b:bytes -> l:list namedGroup
+  -> Tot (result (groups:list namedGroup{List.Tot.length groups = List.Tot.length l + length b / 2}))
+  (decreases (length b))
+let rec parseNamedGroups0 b groups =
+  if length b > 0 then
+    if length b >= 2 then
+      let (ng, bytes) = split b 2 in
+      lemma_split b 2;
+      match parseNamedGroup ng with
+      |Correct ng ->
+        let groups' = ng :: groups in
+        parseNamedGroups0 bytes groups'
+      | Error z    -> Error z
+    else Error (AD_decode_error, perror __SOURCE_FILE__ __LINE__ "")
+  else
+   let grev = List.Tot.rev groups in
+   assume (List.Tot.length grev == List.Tot.length groups);
+   Correct grev
+
+(** Parsing function for a list of named groups *)
+val parseNamedGroups: b:bytes { 2 <= length b /\ length b < 65538 }
+  -> Tot (result (groups:list namedGroup{List.Tot.length groups = (length b - 2) / 2}))
+let parseNamedGroups b =
+  match vlparse 2 b with
+  | Correct b -> parseNamedGroups0 b []
+  | Error z   ->
+    Error(AD_decode_error, perror __SOURCE_FILE__ __LINE__ "Failed to parse named groups")
+
+
+
+
