src/tls/Handshake.Log.fsti
@@ -1,0 +1,158 @@
+module Handshake.Log
+
+// NB still missing regions and modifies clauses.
+
+open Platform.Bytes
+open FStar.Ghost // after HH so as not to shadow reveal :( 
+
+open Hashing
+open Hashing.CRF // now using incremental, collision-resistant, agile Hashing.
+
+module HH = FStar.HyperHeap
+module HS = FStar.HyperStack
+
+type msg = HandshakeMessages.hs_msg 
+
+val format: msg -> Tot bytes 
+val parse_msg: b:bytes -> Tot (option (m:msg {b = format m}))
+
+// No support for binders yet
+
+// Do we compute a hash of the transcript ending with this message?
+// in doubt, we hash! 
+// val tagged: msg -> Tot bool 
+let tagged = 
+  let open HandshakeMessages in function 
+  | Certificate _ -> true // for CertVerify payload in TLS 1.3
+  | CertificateVerify _ -> // for ServerFinish payload in TLS 1.3
+  | Finished _ -> // for 2nd Finished 
+  | ClientHello _ 
+  | ServerHello _ 
+  | EncryptedExtensions _  
+  | ClientKeyExchange _ 
+  | ServerKeyExchange _
+  | ServerHelloDone 
+  | CertificateRequest _
+  | NextProtocol _
+  | HelloRequest  
+  | HelloRetryRequest _ 
+  | SessionTicket _ -> false 
+
+// Does this message complete the flight? 
+// val eoflight: msg -> Tot bool 
+let eoflight = 
+  let open HandshakeMessages in function
+  | ClientKeyExchange _ 
+  | ClientHello _ 
+  | ServerHello _ 
+  | EncryptedExtensions _  
+  | ClientKeyExchange _ 
+  | ServerKeyExchange _
+  | ServerHelloDone 
+  | CertificateRequest _
+  | Certificate _
+  | CertificateVerify _
+  | Finished _
+  | NextProtocol _
+  | HelloRequest  
+  | HelloRetryRequest _ 
+  | SessionTicket _ -> false 
+
+// NB CCS is not explicitly handled here, but can trigger tagging and end-of-flights. 
+
+(* TODO
+- add subregion discipline and the corresponding framing conditions
+- make prior ghost
+- add record-layer calls, keeping track of bytes buffers and their effective lengths
+- support abstract plaintexts and multiple epochs 
+*)
+
+let transcript_bytes ms = List.Tot.fold_left (fun a m -> a @| format m) empty_bytes ms
+// we will need to prove it is injective, we will rely in turn on concrete msg formats
+// should use a named lambda
+
+// formatting of the whole transcript is injective (what about binders?)
+val transcript_format_injective: ms0:list msg -> ms1:list msg -> 
+  Lemma(Seq.equal (transcript_bytes ms0) (transcript_bytes ms1) ==> ms0 == ms1)
+
+val transcript_bytes_append: ms0: list msg -> ms1: list msg -> 
+  Lemma (transcript_bytes (ms0 @ ms1) = transcript_bytes ms0 @| transcript_bytes ms1)
+
+// full specification of the hashed-prefix tags required for a given flight 
+// (in relational style to capture computational-hashed)
+//val tags: a:alg -> prior: list msg -> ms: list msg -> hs: list (tag a) -> Tot Type0 (decreases ms)
+let rec tags (a:alg) (prior: list msg) (ms: list msg) (hs:list (tag a)) : Tot Type0 (decreases ms) = 
+  match ms with 
+  | [] -> hs == [] 
+  | m :: ms -> 
+      let prior = prior @ [m] in
+      match tagged m, hs with 
+      | true, h::hs -> let t = transcript_bytes prior in (hashed a t /\ h == hash a t /\ tags a prior ms hs)
+      | false, hs -> tags a prior ms hs
+      | _ -> False 
+
+val tags_append: a:alg -> prior: list msg -> ms0: list msg -> ms1: list msg -> hs0: list (tag a) -> hs1: list (tag a) ->
+  Lemma (tags a prior ms0 hs0 /\ tags a (prior @ ms0) ms1 hs1 ==> tags a prior (ms0 @ ms1) (hs0 @ hs1))
+
+
+(* STATE *)
+
+type t (r:HH.rid) (a:alg) 
+//17-03-25 assume new warning?
+
+//  specification-level transcript of all handshake messages logged so far
+val transcriptT: h:HS.mem -> #region:HH.rid -> #a:alg -> t region a -> GTot (list msg) 
+
+// specification-level guard for sending: we have not started receiving the next flight
+val writing: h:HS.mem -> #region:HH.rid -> #a:alg -> t region a -> GTot bool 
+
+val create: region:HH.rid -> a:alg -> ST (t region a) 
+  (requires (fun h0 -> True))
+  (ensures (fun h0 r h1 -> // "allocated in r" /\ writing h1 r /\ 
+    writing h1 r /\  
+    transcriptT h1 r == []))
+  
+// We send one message at a time (or in two steps for CH); 
+// for call-site simplicity we distinguish between tagged and untagged messages
+// We require ms_0 be empty; otherwise the hash computation is messed up
+
+// We do not enforce "tagged m", a local decision 
+
+val send: #region:HH.rid -> #a:alg -> r:t region a -> m:msg (*{~(tagged m)}*) -> ST unit 
+  (requires (fun h0 -> writing h0 r )) 
+  (ensures (fun h0 _ h1 -> 
+    writing h1 r /\
+    transcriptT h1 r == transcriptT h0 r @ [m]  ))
+
+val send_tag: #region:HH.rid -> #a:alg -> r:t region a -> m:msg (*{tagged m}*) -> ST (tag a)
+  (requires (fun h0 -> writing h0 r )) 
+  (ensures (fun h0 h h1 -> 
+    let t_0 = transcriptT h0 r in 
+    let t_1 = transcriptT h1 r in 
+    let bs = transcript_bytes t_1 in
+    writing h1 r /\
+    t_1 == t_0 @ [m] /\
+    hashed a bs /\ h == hash a bs ))
+
+// We receive messages in whole flights; 
+// note that, untill a full flight is received, we lose "writing h1 r"
+val receive: #region:HH.rid -> #a:alg -> r:t region a -> bytes -> ST (option (list msg * list (tag a)))
+  (requires (fun h0 -> True))
+  (ensures (fun h0 o h1 -> 
+    let t0 = transcriptT h0 r in
+    let t1 = transcriptT h1 r in
+    match o with 
+    | Some (ms, hs) -> t1 == t0 @ ms /\ tags a t0 ms hs /\ writing h1 r
+    | None -> t1 == t0 ))
+
+// We receive CCS as external end-of-flight signals;
+// we return the messages processed so far, and their final tag; 
+// we still can't write.
+// This should *fail* if there are pending input bytes. 
+val receiveCCS: #region:HH.rid -> #a:alg -> r:t region a -> ST (list msg * list (tag a) * tag a)
+  (requires (fun h0 -> True))
+  (ensures (fun h0 (ms,hs,h) h1 -> 
+    let t0 = transcriptT h0 r in
+    let t1 = transcriptT h1 r in
+    let tr = transcript_bytes t1 in 
+    t1 == t0 @ ms /\ tags a t0 ms hs /\ hashed a tr /\ h = hash a tr ))
